theories/base_logic/lib/invariants.v
@@ -110,12 +110,11 @@ Qed.
 Global Instance into_inv_inv N P : IntoInv (inv N P) N.
 
 Global Instance elim_inv_inv E N P Q Q' :
-  (∀ R, ElimModal True false false (|={E,E∖↑N}=> R) R Q Q') →
-  ElimInv (↑N ⊆ E) (inv N P) True (▷ P) (▷ P ={E∖↑N,E}=∗ True) Q Q'.
+  InvOpener E (E∖↑N) (▷ P) (▷ P) None Q Q' →
+  ElimInv (↑N ⊆ E) (inv N P) True (▷ P) Q Q'.
 Proof.
-  rewrite /ElimInv /ElimModal. iIntros (Helim ?) "(#H1&_&H2)".
-  iApply (Helim with "[H2]"); [done|]; simpl. iSplitR "H2"; [|done].
-  iMod (inv_open _ N with "[#]") as "(HP&Hclose)"; auto with iFrame.
+  rewrite /ElimInv /InvOpener. iIntros (Hopener ?) "(#Hinv & _ & Hcont)".
+  iApply (Hopener with "Hcont"). iApply inv_open; done.
 Qed.
 
 Lemma inv_open_timeless E N P `{!Timeless P} :
