theories/program_logic/weakestpre.v
@@ -404,4 +404,26 @@ Section proofmode_classes.
   Global Instance add_modal_fupd_wp s E e P Φ :
     AddModal (|={E}=> P) P (WP e @ s; E {{ Φ }}).
   Proof. by rewrite /AddModal fupd_frame_r wand_elim_r fupd_wp. Qed.
+
+  Global Instance inv_opener_wp E1 E2 P P' (P'' : option _) e s Φ :
+    Atomic (stuckness_to_atomicity s) e →
+    InvOpener E1 E2 P P' P'' (WP e @ s; E1 {{ Φ }})
+              (WP e @ s; E2 {{ v, P' ∗ coq_tactics.maybe_wand P'' (Φ v) }})%I.
+  Proof.
+    intros ?. rewrite /InvOpener. setoid_rewrite coq_tactics.maybe_wand_sound.
+    iIntros "Hinner >[HP Hclose]".
+    iApply (wp_wand with "[Hinner HP]"); first by iApply "Hinner".
+    iIntros (v) "[HP HΦ]". iApply "HΦ". by iApply "Hclose".
+  Qed.
+
+  Global Instance inv_opener_wp_nonatomic E P P' (P'' : option _) e s Φ :
+    InvOpener E E P P' P'' (WP e @ s; E {{ Φ }})
+              (WP e @ s; E {{ v, P' ∗ coq_tactics.maybe_wand P'' (Φ v) }})%I.
+  Proof.
+    rewrite /InvOpener. setoid_rewrite coq_tactics.maybe_wand_sound.
+    iIntros "Hinner >[HP Hclose]". iApply wp_fupd.
+    iApply (wp_wand with "[Hinner HP]"); first by iApply "Hinner".
+    iIntros (v) "[HP HΦ]". iApply "HΦ". by iApply "Hclose".
+  Qed.
+
 End proofmode_classes.
